

Review for Exam 2

1. Sample problems

Problem 1:

- Give an example of a function $f : \mathbb{Z} \rightarrow \mathbb{Z}$ which is injective but not surjective.
- Give an example of a function $g : \mathbb{Z} \rightarrow \mathbb{Z}$ which is surjective but not injective.

Solution for 1a:

Let $f : \mathbb{Z} \rightarrow \mathbb{Z}$ be given by the rule $f(x) = 2x$. The image of f is the set of even integers, which is a proper subset of \mathbb{Z} ; thus f is not surjective. But f is injective: if $x, x' \in \mathbb{Z}$ and $f(x) = f(x')$ then $2x = 2x'$. Cancellation of the factor 2 then implies that $x = x'$. This demonstrates that f is injective.

Solution for 1b:

Let $g : \mathbb{Z} \rightarrow \mathbb{Z}$ be given by the rule

$$g(x) = \begin{cases} x & \text{if } x \geq 0 \\ x + 1 & \text{if } x < 0 \end{cases}$$

Note that $g(0) = g(-1) = 0$; this shows that g is *not injective*. On the other hand, let $y \in \mathbb{Z}$. If $y \geq 0$ then $y = g(y)$ while if $y < 0$ then $y = g(y - 1)$. This shows that g is *surjective*.

Problem 2: We have seen that for finite sets A and B , we have

$$(\heartsuit) \quad |A \cup B| = |A| + |B| - |A \cap B|.$$

Now, let A, B, C be finite sets.

- Suppose that

$$|A \cup B \cup C| = |A| + |B| + |C|.$$

Prove that $A \cap B = \emptyset$, $A \cap C = \emptyset$ and $B \cap C = \emptyset$.

- If $A \cap B \cap C = \emptyset$, is it true that $|A \cup B \cup C| = |A| + |B| + |C|$? Justify your response with a proof or a counter-example.

Solution for 2a:

Note that $A \cup B \cup C = A \cup (B \cup C)$. Thus (♥) shows that

$$|A \cup B \cup C| = |A| + |B \cup C| - |A \cap (B \cup C)|.$$

Another application of (♥) shows that $|B \cup C| = |B| + |C| - |B \cap C|$.

Thus we find

$$|A \cup B \cup C| = |A| + |B| + |C| - |B \cap C| - |A \cap (B \cup C)|.$$

Since $|A \cup B \cup C| = |A| + |B| + |C|$ by hypothesis, and since for any finite set, $|X|$ is non-negative, we now deduce that $|B \cap C| = 0$ and $|A \cap (B \cup C)| = 0$. In particular, $B \cap C = \emptyset$.

Now, $A \cap (B \cup C) = (A \cap B) \cup (A \cap C)$. A further application of (♥) now shows that

$$(*) \quad 0 = |A \cap (B \cup C)| = |(A \cap B) \cup (A \cap C)| = |A \cap B| + |A \cap C| - |(A \cap B) \cap (A \cap C)|.$$

Since $B \cap C = \emptyset$, we know that $(A \cap B) \cap (A \cap C) = \emptyset$. Thus (*) shows that

$$0 = |A \cap B| + |A \cap C|.$$

Thus $A \cap B = A \cap C = \emptyset$ as required.

Solution for 2b:

It is not true that $A \cap B \cap C = \emptyset \Rightarrow |A \cup B \cup C| = |A| + |B| + |C|$.

Indeed, let $A = \{1, 2\}$, $B = \{2, 3\}$, $C = \{3, 4\}$. Then $A \cap B \cap C = \emptyset$. But $A \cup B \cup C = \{1, 2, 3, 4\}$ so that

$$|A \cup B \cup C| = 4 < 6 = |A| + |B| + |C|.$$

Problem 3: Let S be a finite set having $n \in \mathbb{N}$ elements, let $d \in \mathbb{N}$.

A **sequence** of elements of S of length d is a list a_0, a_1, \dots, a_{d-1} where $a_j \in S$ for each j .

Let $T_{\leq d}$ be the set of all sequences of elements of S of length $\leq d$.

Give an expression for the cardinality $|T_{\leq d}|$ in terms of d and n .

Solution for 3:

The number of sequences of elements of S of length equal to d is given by n^d , since there are n choices for each of the d entries in the sequence.

$$\text{Now, } |T_{\leq d}| = \sum_{i=1}^d n^i.$$

Problem 4: Let $f : X \rightarrow Y$ be a function. Define a relation \sim on X by the rule: $x \sim x'$ if and only if $f(x) = f(x')$.

- a. Show that \sim is an equivalence relation.
- b. For $x \in X$, show that the equivalence class $[x]$ is equal to $f^{-1}(f(x))$.

Solution for 4:

- a.
 - reflexive: If $x \in X$, then $f(x) = f(x) \Rightarrow x \sim x$.
 - symmetric: For $x, y \in X$, $x \sim y \Rightarrow f(x) = f(y) \Rightarrow f(y) = f(x) \Rightarrow y \sim x$.
 - transitive: For $x, y, z \in X$,

$$\begin{aligned} x \sim y \text{ and } y \sim z &\Rightarrow f(x) = f(y) \text{ and } f(y) = f(z) \\ &\Rightarrow f(x) = f(z) \Rightarrow x \sim z. \end{aligned}$$

- b. Recall that $[x] = \{z \in X \mid x \sim z\}$ and $f^{-1}(f(x)) = \{z \in X \mid f(x) = f(z)\}$.

We now see that $[x] = f^{-1}(f(x))$. Indeed, for $z \in X$ we have

$$z \in [x] \Leftrightarrow x \sim z \Leftrightarrow f(x) = f(z) \Leftrightarrow z \in f^{-1}(f(x)).$$

Problem 5: Let $n \in \mathbb{N}$ and write $\mathbb{Z}^2 = \mathbb{Z} \times \mathbb{Z}$. For $(a, b), (a', b') \in \mathbb{Z}^2$ we consider the relation

$$(a, b) \equiv (a', b') \pmod{n} \text{ provided that } a \equiv a' \pmod{n} \text{ and } b \equiv b' \pmod{n}.$$

- a. Show that this relation is an equivalence relation on \mathbb{Z}^2 .
- b. Show that there are n^2 equivalence classes in \mathbb{Z}^2 for this relation.

Solution for 5:

- a. • reflexive: For $(a, b) \in \mathbb{Z}^2$, $a \equiv a \pmod{n}$ and $b \equiv b \pmod{n}$ since $\equiv \pmod{n}$ is an equivalence relation on \mathbb{Z} . Thus $(a, b) \sim (a, b)$.
• symmetric: Let $(a, b), (c, d) \in \mathbb{Z}^2$ and suppose that $(a, b) \sim (c, d)$. Since $\equiv \pmod{n}$ is a symmetric relation on \mathbb{Z} , we see that

$$a \equiv c \pmod{n} \text{ and } b \equiv d \pmod{n} \Rightarrow c \equiv a \pmod{n} \text{ and } d \equiv b \pmod{n}.$$

This now shows that $(c, d) \sim (a, b)$.

- transitive: Let $(a, b), (c, d), (e, f) \in \mathbb{Z}^2$ with $(a, b) \sim (c, d)$ and $(c, d) \sim (e, f)$.

The first assumption shows that

$$a \equiv c \pmod{n} \text{ and } b \equiv d \pmod{n},$$

and the second assumption shows that

$$c \equiv e \pmod{n} \text{ and } d \equiv f \pmod{n}.$$

Since $\equiv \pmod{n}$ is a transitive relation on \mathbb{Z} , we deduce that

$$a \equiv e \pmod{n} \text{ and } b \equiv f \pmod{n}.$$

This confirms that $(a, b) \sim (e, f)$ as required.

- b. Recall that we write \mathbb{Z}_n for the set of equivalence class in \mathbb{Z} for the relation $\equiv \pmod{n}$. We know that $|\mathbb{Z}_n| = n$.

I claim that the set X of equivalence classes for \sim in \mathbb{Z}^2 is in bijection with $\mathbb{Z}_n \times \mathbb{Z}_n$. Once this bijection is established, it follows that the number of equivalence classes is given by $|X| = |\mathbb{Z}_n \times \mathbb{Z}_n| = n \cdot n = n^2$.

Now, define $f : X \rightarrow \mathbb{Z}_n \times \mathbb{Z}_n$ by the rule $f([(a, b)]) = ([a]_n, [b]_n)$ for $(a, b) \in \mathbb{Z}^2$.

We must confirm that f is *well-defined*. Well, if $(a, b) \sim (c, d)$ we must argue that $f([(a, b)]) = f([(c, d)])$. But $(a, b) \sim (c, d)$ implies that $a \equiv c \pmod{n}$ and $b \equiv d \pmod{n}$ and this shows that $[a]_n = [c]_n$ and $[b]_n = [d]_n$. Thus $f([(a, b)]) = ([a]_n, [b]_n) = ([c]_n, [d]_n) = f([(c, d)])$.

On the other hand, we define $g : \mathbb{Z}_n \times \mathbb{Z}_n \rightarrow X$ by the rule $g([a]_n, [b]_n) = [(a, b)]$. Again we must argue that g is well-defined. Suppose $([a]_n, [b]_n) = ([c]_n, [d]_n)$ is an equality in $\mathbb{Z}_n \times \mathbb{Z}_n$. Thus $[a]_n = [c]_n$ and $[b]_n = [d]_n$. But this shows that $(a, b) \sim (c, d)$ so that $[(a, b)] = [(c, d)]$ in X , confirming that g is well-defined.

Now, by definition we have

$$(f \circ g)([a]_n, [b]_n) = f([(a, b)]) = ([a]_n, [b]_n) \text{ so that } f \circ g = \text{id}_{\mathbb{Z}_n \times \mathbb{Z}_n}$$

and

$$(g \circ f)([(a, b)]) = g([a]_n, [b]_n) = [(a, b)] \text{ so that } g \circ f = \text{id}_X.$$

Thus f is a bijection $X \rightarrow \mathbb{Z}_n \times \mathbb{Z}_n$.

Problem 6: Let A and B be sets.

- If A is finite and B is countably infinite, prove that the union $A \cup B$ is a countably infinite set.
- Prove that there is a bijection between $A \sqcup A \sqcup A$ and $A \times \{0, 1, 2\}$.
- Let $f : A \rightarrow B$ be an injective function, and suppose that A is infinite and not countable. Prove that B is infinite and not countable.

Solution for 6a:

- Choosing a bijection between A and $I_n = \{0, 1, \dots, n-1\}$ and a bijection between B and \mathbb{N} , we are reduced to prove that $I_n \sqcup \mathbb{N}$ is countably infinite. We just need to demonstrate a bijection between $I_n \sqcup \mathbb{N}$ and \mathbb{N} .

Define $f : I_n \sqcup \mathbb{N} \rightarrow \mathbb{N}$ by the rule

$$f(x) = \begin{cases} x & \text{if } x \in I_n \\ x + n & \text{otherwise.} \end{cases}$$

We argue that f is surjective. If $m \in \mathbb{N}$ and $m \geq n$, then $m - n \in \mathbb{N} \subset I_n \sqcup \mathbb{N}$, and $m = f(m - n)$.

If $m < n$ then $m \in I_n \subset I_n \sqcup \mathbb{N}$, and $m = f(m)$.

This shows in all cases that f is surjective.

Finally, we argue that f is injective. Before proceeding, we observe that for $x \in I_n \sqcup \mathbb{N}$ we have by definition:

$$(\heartsuit) : f(x) \in I_n \subset \mathbb{N} \text{ if and only if } x \in I_n \subset I_n \sqcup \mathbb{N}.$$

For this, suppose that $x, y \in I_n \sqcup \mathbb{N}$ and assume that $f(x) = f(y)$. If $f(x) = f(y) \in I_n$ observation (\heartsuit) shows that $x, y \in I_n$. Now the definition of f shows that $x = y$.

If $f(x) = f(y) \notin I_n$, then $x, y \in \mathbb{N} \subset I_n \sqcup \mathbb{N}$ so that

$$f(x) = f(y) \Rightarrow x + n = y + n \Rightarrow x = y.$$

This shows in all cases that f is injective.

Since f is bijective, $I_n \sqcup \mathbb{N}$ is indeed countably infinite.

Solution for 6b:

An element $x \in A \sqcup A \sqcup A$ is either in the left, middle or right-hand copy of A . We define

$$f : A \sqcup A \sqcup A \rightarrow A \times \{0, 1, 2\}$$

by the rule

$$f(x) = \begin{cases} (x, 0) & \text{if } x \text{ is in the left-hand copy of } A \\ (x, 1) & \text{if } x \text{ is in the middle copy of } A \\ (x, 2) & \text{if } x \text{ is in the right-hand copy of } A \end{cases}.$$

Then f is a bijection. (**NB:** recall that we **defined** the disjoint union using a product construction, so this problem is more-or-less just an invocation of the definition of the disjoint union.)

Solution for 6c:

We prove the contra-positive. Thus, we suppose the negation of “ B is infinite and not countable.” Thus we suppose: B is finite or countably infinite.

And we must prove the negation of “ A is infinite and not countable.” This we must prove: A is finite or countably infinite.

Now the required result just follows from the (given) observation (i) in problem 7.

Problem 7: We showed the following in class (and you may use these statements here):

Let A, B be sets.

- i. If $f : A \rightarrow B$ is an injective function and if B is countable, then A is either finite or countably infinite.
- ii. If $g : B \rightarrow A$ is a surjective function and if A is countable, then B is either finite or countably infinite.
- a. Prove that if A is a countably infinite set and if \sim is an equivalence relation on A , then the set of equivalence classes is either finite or countably infinite.
- b. Show by example for some countable set(s) A with equivalence relation(s) \sim that the set B of equivalence classes can be finite, and that B can be infinite.

Solution for 7:

- a. Let X be the set of equivalence classes in A for the eq. relation \sim . There is a surjective function $f : A \rightarrow X$ given by $f(a) = [a]$. Since A is countably infinite, it follows from (ii) that X is countable infinite or finite, as required.
- b. Note that \mathbb{Z} is countably infinite. For any $n \in \mathbb{N}_{>0}$, the set of equivalence classes \mathbb{Z}_n for the equivalence relation $\equiv (\text{mod } n)$ is finite, since $|\mathbb{Z}_n| = n$.

On the other hand, take the trivial equivalence relation on \mathbb{Z} just defined by equality: $x \sim y \Leftrightarrow x = y$. Then for each $x \in \mathbb{Z}$, the equivalence class $[x]$ is just the singleton set $\{x\}$. In particular, the set of equivalence classes is in bijection with \mathbb{Z} and is hence (countably) infinite.

Problem 8: Find all solutions x to the following equations in \mathbb{Z}_{14} :

- a. $[3]_{14} \cdot x + [2]_{14} = [6]_{14}$
(Note that $[3]_{14} \cdot [5]_{14} = [15]_{14} = [1]_{14}$.)
- b. $[2]_{14} \cdot x = [2]_{14}$.

Solution for 8:

- a. We need $[3] \cdot x = [4]$ in \mathbb{Z}_{14} . Since $[3] \cdot [5] = [1]$ in \mathbb{Z}_{14} , we see that the only solution is
$$x = [5] \cdot [3]x = [5] \cdot [4] = [20]_{14} = [6]_{14}.$$
- b. To solve $[2] \cdot x = [2]$ in \mathbb{Z}_{14} , we can write $x = [z]$ for some $z \in \mathbb{Z}$ with $0 \leq z < 14$. Then $[2] \cdot x = [2z]$. So we must decide: for which z is $2z \equiv 2(\text{mod } 14)$?
We of course have the “obvious” solution $x = [1]_{14}$ (i.e. $z = 1$.)
Note that $2z < 28$, and the integers between 0 and 28 which are $\equiv 2(\text{mod } 14)$ are precisely: 2 and 16.
So: there is one further solution, namely: $x = [z] = [8]_{14}$.
So the full set of solutions is: $[1]_{14}$ and $[8]_{14}$.

Problem 9: Let $n \in \mathbb{N}$ and consider the mapping $f : \mathbb{Z}_n \rightarrow \mathbb{Z}_n$ given by $f([x]_n) = [x]_n \cdot [x]_n$.

- a. Show that f is well-defined.
(We obtained a result in class that implies that f is well-defined, but show the details here).
- b. Is f injective? Is f surjective? Prove or disprove each statement.

Solution for 9:

- a. Suppose that $[x]_n = [y]_n$ for $x, y \in \mathbb{Z}$ -i.e. that $x \equiv y \pmod{n}$. To see that f is well-defined, we need to check that $f([x]) = f([y])$. Now, $f([x]) = [x] \cdot [x] = [x^2]$. So we must argue that $x^2 \equiv y^2 \pmod{n}$. Let's write $x - y = k \cdot n$ for $k \in \mathbb{Z}$.

Then we have

$$x^2 - y^2 = (x - y)(x + y) = k \cdot n \cdot (x + y) \Rightarrow n \mid x^2 - y^2 \Rightarrow x^2 \equiv y^2 \pmod{n}.$$

This proves that f is indeed well-defined.

- b. In general, f is neither surjective nor injective.

For example, if $n = 3$, then

$$f([0]) = [0], f([1]) = [1], f([2]) = [4]_3 = [1]_3.$$

Thus the image of f is $\{[0], [1]\}$ so that f is not surjective.

Moreover, $f([1]) = f([2])$ but $[1] \neq [2]$ so that f is not injective.

Problem 10: Assume that a_n is a sequence with $\lim_{n \rightarrow \infty} a_n = 1$. Prove that $(-1)^n a_n$ is not a Cauchy sequence.

Solution for 10:

Since a_n converges to 1, we may find $m_0 \in \mathbb{N}$ such that $n \geq m_0 \Rightarrow |a_n - 1| < 1/2$. Thus

$$-1/2 < a_n - 1 < 1/2 \Rightarrow 1/2 < a_n.$$

We now show that the sequence $(-1)^n \cdot a_n$ fails to be Cauchy.

We must prove that (\clubsuit): $\exists \varepsilon > 0$ such that $\forall m \in \mathbb{N}, \exists n_1, n_2 \geq m$ such that

$$|(-1)^{n_1} \cdot a_{n_1} - (-1)^{n_2} \cdot a_{n_2}| \geq \varepsilon.$$

We take $\varepsilon = 1/2$. For any m , choose $n_1, n_2 \geq \max(m, m_0)$ with n_1 even and n_2 odd. Observe that $(-1)^{n_1} \cdot a_{n_1} = a_{n_1}$ and $(-1)^{n_2} \cdot a_{n_2} = -a_{n_2}$.

Then we have

$$|(-1)^{n_1} a_{n_1} - (-1)^{n_2} \cdot a_{n_2}| = |a_{n_1} + a_{n_2}| \geq |a_{n_1}| > 1/2.$$

This confirms (\clubsuit) and shows that $(-1)^n \cdot a_n$ is not Cauchy.

Problem 11: If a_n is a Cauchy sequence, prove that the sequence $b_n = a_n \cdot a_{2n}$ is a Cauchy sequence.

(You can use results from class/the notes - just give a brief description of the result you are using).

Solution for 11:

We know that the product of Cauchy sequences is again a Cauchy sequence. Thus to prove that b_n is Cauchy it is enough to know that a_n is Cauchy – which is true by hypothesis – and that a_{2n} is Cauchy.

Thus, it remains only to prove that a_{2n} is Cauchy.

Let $\varepsilon > 0$. Since a_n is Cauchy, we may choose $m \in \mathbb{N}$ such that

$$(*) : n_1, n_2 \geq m \Rightarrow |a_{n_1} - a_{n_2}| < \varepsilon.$$

Now for any $n_1, n_2 \geq m$, notice that $2n_1 \geq m$ and $2n_2 \geq m$.

Thus $(*)$ implies that

$$|a_{2n_1} - a_{2n_2}| < \varepsilon.$$

This confirms that a_{2n} is Cauchy.